src/cddl/pulse/CDDL.Pulse.Parse.ArrayGroup.fst
@@ -1,0 +1,268 @@
+module CDDL.Pulse.Parse.ArrayGroup
+include CDDL.Pulse.ArrayGroup
+include CDDL.Pulse.Parse.Base
+open Pulse.Lib.Pervasives
+open CBOR.Spec.API.Type
+open CBOR.Pulse.API.Base
+module Trade = Pulse.Lib.Trade.Util
+module R = Pulse.Lib.Reference
+
+let impl_zero_copy_array_group_precond
+  (t: array_group None)
+  (l: list cbor)
+: Tot prop
+= t l == Some (l, [])
+
+let impl_zero_copy_array_group_postcond
+  (#t: array_group None)
+  (#tgt: Type0)
+  (#tgt_size: tgt -> nat)
+  (#tgt_serializable: tgt -> bool)
+  (ps: array_group_parser_spec t tgt_size tgt_serializable)
+  (l: list cbor)
+  (v: tgt)
+: Tot prop
+= t l == Some (l, []) /\
+  ps l == v
+
+inline_for_extraction noextract [@@noextract_to "krml"]
+let impl_zero_copy_array_group
+  (#cbor_array_iterator_t: Type)
+  (cbor_array_iterator_match: perm -> cbor_array_iterator_t -> list cbor -> slprop)
+    (#t: array_group None)
+    (#tgt: Type0)
+    (#tgt_size: tgt -> nat)
+    (#tgt_serializable: tgt -> bool)
+    (ps: array_group_parser_spec t tgt_size tgt_serializable)
+    (#impl_tgt: Type0)
+    (r: rel impl_tgt tgt)
+=
+    (pc: R.ref cbor_array_iterator_t) ->
+    (#c: Ghost.erased cbor_array_iterator_t) ->
+    (#p: perm) ->
+    (#l: Ghost.erased (list cbor)) ->
+    stt impl_tgt
+        (R.pts_to pc c **
+          cbor_array_iterator_match p c l **
+          pure (impl_zero_copy_array_group_precond t l)
+        )
+        (fun res -> exists* v c' .
+          r res v **
+          R.pts_to pc c' **
+          Trade.trade
+            (r res v)
+            (cbor_array_iterator_match p c l) **
+          pure (impl_zero_copy_array_group_postcond ps l v)
+        )
+
+inline_for_extraction noextract [@@noextract_to "krml"]
+```pulse
+fn impl_zero_copy_array
+  (#ty: Type0)
+  (#vmatch: perm -> ty -> cbor -> slprop)
+  (#cbor_array_iterator_t: Type)
+  (#cbor_array_iterator_match: perm -> cbor_array_iterator_t -> list cbor -> slprop)
+  (cbor_array_iterator_start: array_iterator_start_t vmatch cbor_array_iterator_match)
+    (#t: Ghost.erased (array_group None))
+    (#tgt: Type0)
+    (#tgt_size: Ghost.erased (tgt -> nat))
+    (#tgt_serializable: Ghost.erased (tgt -> bool))
+    (#ps: Ghost.erased (array_group_parser_spec t tgt_size tgt_serializable))
+    (#impl_tgt: Type0)
+    (#r: rel impl_tgt tgt)
+    (pa: impl_zero_copy_array_group cbor_array_iterator_match ps r)
+: impl_zero_copy_parse #ty vmatch #(t_array (Ghost.reveal t)) #tgt #(spec_array_group_serializable (Ghost.reveal tgt_size) (Ghost.reveal tgt_serializable)) (parser_spec_array_group (Ghost.reveal ps) (spec_array_group_serializable (Ghost.reveal tgt_size) (Ghost.reveal tgt_serializable))) #impl_tgt r
+=
+  (c: _)
+  (#p: _)
+  (#v: _)
+{
+  let ar = cbor_array_iterator_start c;
+  // BEGIN FIXME: change the type of l1 in the signature of cbor_array_iterator_start
+  with pl (l1: list cbor) . assert (cbor_array_iterator_match pl ar l1);
+  let l : Ghost.erased (list cbor) = Ghost.hide l1;
+  Trade.rewrite_with_trade (cbor_array_iterator_match pl ar l1)
+    (cbor_array_iterator_match pl ar l);
+  Trade.trans _ _ (vmatch p c v);
+  // END FIXME
+  let mut a = ar;
+  let res = pa a;
+  Trade.trans _ _ (vmatch p c v);
+  res
+}
+```
+
+inline_for_extraction noextract [@@noextract_to "krml"]
+```pulse
+fn impl_zero_copy_array_group_item
+  (#ty: Type0)
+  (#vmatch: perm -> ty -> cbor -> slprop)
+  (#cbor_array_iterator_t: Type)
+  (#cbor_array_iterator_match: perm -> cbor_array_iterator_t -> list cbor -> slprop)
+  (cbor_array_iterator_next: array_iterator_next_t vmatch cbor_array_iterator_match)
+    (#t: Ghost.erased typ)
+    (#tgt: Type0)
+    (#tgt_serializable: Ghost.erased (tgt -> bool))
+    (#ps: Ghost.erased (parser_spec t tgt tgt_serializable))
+    (#impl_tgt: Type0)
+    (#r: rel impl_tgt tgt)
+    (pa: impl_zero_copy_parse vmatch ps r)
+: impl_zero_copy_array_group #cbor_array_iterator_t cbor_array_iterator_match #(array_group_item (Ghost.reveal t)) #tgt #(ag_spec_item_size tgt) #(Ghost.reveal tgt_serializable) (array_group_parser_spec_item (Ghost.reveal ps) (ag_spec_item_size tgt)) #impl_tgt r
+=
+  (pc: _)
+  (#c: _)
+  (#p: _)
+  (#l: _)
+{
+  let x = cbor_array_iterator_next pc;
+  Trade.elim_hyp_r _ _ _;
+  let res = pa x;
+  Trade.trans _ _ (cbor_array_iterator_match p c l);
+  res
+}
+```
+
+module U64 = FStar.UInt64
+
+let list_append_length_pat
+  (#t: Type)
+  (l1 l2: list t)
+: Lemma
+  (ensures (List.Tot.length (List.Tot.append l1 l2) == List.Tot.length l1 + List.Tot.length l2))
+  [SMTPat (List.Tot.append l1 l2)]
+= List.Tot.append_length l1 l2
+
+inline_for_extraction noextract [@@noextract_to "krml"]
+```pulse
+fn impl_zero_copy_array_group_concat
+  (#cbor_array_iterator_t: Type)
+  (#cbor_array_iterator_match: perm -> cbor_array_iterator_t -> list cbor -> slprop)
+  (length: array_iterator_length_t cbor_array_iterator_match)
+  (share: array_iterator_share_t cbor_array_iterator_match)
+  (gather: array_iterator_gather_t cbor_array_iterator_match)
+  (truncate: array_iterator_truncate_t cbor_array_iterator_match)
+    (#t1: Ghost.erased (array_group None))
+    (#tgt1: Type0)
+    (#tgt_size1: Ghost.erased (tgt1 -> nat))
+    (#tgt_serializable1: Ghost.erased (tgt1 -> bool))
+    (#ps1: Ghost.erased (array_group_parser_spec t1 tgt_size1 tgt_serializable1))
+    (#impl_tgt1: Type0)
+    (#r1: rel impl_tgt1 tgt1)
+    (pa1: impl_zero_copy_array_group cbor_array_iterator_match ps1 r1)
+    (v1: impl_array_group cbor_array_iterator_match t1)
+    (#t2: Ghost.erased (array_group None))
+    (#tgt2: Type0)
+    (#tgt_size2: Ghost.erased (tgt2 -> nat))
+    (#tgt_serializable2: Ghost.erased (tgt2 -> bool))
+    (#ps2: Ghost.erased (array_group_parser_spec t2 tgt_size2 tgt_serializable2))
+    (#impl_tgt2: Type0)
+    (#r2: rel impl_tgt2 tgt2)
+    (pa2: impl_zero_copy_array_group cbor_array_iterator_match ps2 r2)
+    (sq: squash (
+      array_group_concat_unique_weak t1 t2
+    ))
+: impl_zero_copy_array_group #cbor_array_iterator_t cbor_array_iterator_match #(array_group_concat (Ghost.reveal t1) (Ghost.reveal t2)) #(tgt1 & tgt2) #(ag_spec_concat_size (Ghost.reveal tgt_size1) (Ghost.reveal tgt_size2)) #(ag_spec_concat_serializable (Ghost.reveal tgt_serializable1) (Ghost.reveal tgt_serializable2)) (array_group_parser_spec_concat (Ghost.reveal ps1) (Ghost.reveal ps2) (ag_spec_concat_size (Ghost.reveal tgt_size1) (Ghost.reveal tgt_size2)) (ag_spec_concat_serializable (Ghost.reveal tgt_serializable1) (Ghost.reveal tgt_serializable2))) #(impl_tgt1 & impl_tgt2) (rel_pair r1 r2)
+=
+  (pc: _)
+  (#gc: _)
+  (#p: _)
+  (#l: _)
+{
+  let gl = Ghost.hide (Some?.v (Ghost.reveal t1 l));
+  let gl1 = Ghost.hide (fst gl);
+  let gl2 = Ghost.hide (snd gl);
+  CBOR.Spec.Util.list_splitAt_append_elim gl1 gl2;
+  let c0 = !pc;
+  Trade.rewrite_with_trade
+    (cbor_array_iterator_match p gc l)
+    (cbor_array_iterator_match p c0 l); // FIXME: WHY WHY WHY? variable as head symbol
+  let rlen0 = length c0;
+  share c0;
+  ghost fn aux (_: unit)
+  requires emp ** (cbor_array_iterator_match (p /. 2.0R) c0 l ** cbor_array_iterator_match (p /. 2.0R) c0 l)
+  ensures cbor_array_iterator_match p c0 l
+  {
+    gather c0 #(p /. 2.0R) #l #(p /. 2.0R) #l;
+    rewrite (cbor_array_iterator_match (p /. 2.0R +. p /. 2.0R) c0 l)
+      as (cbor_array_iterator_match p c0 l)
+  };
+  Trade.intro _ _ _ aux;
+  Trade.trans _ _ (cbor_array_iterator_match p gc l);
+  let _tmp = v1 pc;
+  assert (pure (_tmp));
+  with p1 gc1 l1 . assert (pts_to pc gc1 ** cbor_array_iterator_match p1 gc1 l1);
+  Trade.trans_hyp_r _ _ _ _;
+  let c1 = !pc;
+  Trade.rewrite_with_trade (cbor_array_iterator_match p1 gc1 l1)
+    (cbor_array_iterator_match p1 c1 l1);
+  Trade.trans_hyp_r _ _ _ _;
+  let rlen1 = length c1;
+  assert (pure (U64.v rlen1 <= U64.v rlen0));
+  let c0' = truncate c0 (rlen0 `U64.sub` rlen1);
+  Trade.trans_hyp_l _ _ _ _;
+  pc := c0';
+  let w1 = pa1 pc;
+  Trade.trans_hyp_l _ _ _ _;
+  pc := c1;
+  let w2 = pa2 pc;
+  Trade.trans_hyp_r _ _ _ _;
+  with z1 z2 . assert (r1 w1 z1 ** r2 w2 z2);
+  let res = (w1, w2);
+  Trade.rewrite_with_trade
+    (r1 w1 z1 ** r2 w2 z2)
+    (rel_pair r1 r2 res (z1, z2));
+  Trade.trans (rel_pair r1 r2 res (z1, z2)) _ _;
+  res
+}
+```
+
+inline_for_extraction noextract [@@noextract_to "krml"]
+```pulse
+fn impl_zero_copy_array_group_choice
+  (#cbor_array_iterator_t: Type)
+  (#cbor_array_iterator_match: perm -> cbor_array_iterator_t -> list cbor -> slprop)
+    (#t1: Ghost.erased (array_group None))
+    (#tgt1: Type0)
+    (#tgt_size1: Ghost.erased (tgt1 -> nat))
+    (#tgt_serializable1: Ghost.erased (tgt1 -> bool))
+    (#ps1: Ghost.erased (array_group_parser_spec t1 tgt_size1 tgt_serializable1))
+    (#impl_tgt1: Type0)
+    (#r1: rel impl_tgt1 tgt1)
+    (pa1: impl_zero_copy_array_group cbor_array_iterator_match ps1 r1)
+    (v1: impl_array_group cbor_array_iterator_match t1)
+    (#t2: Ghost.erased (array_group None))
+    (#tgt2: Type0)
+    (#tgt_size2: Ghost.erased (tgt2 -> nat))
+    (#tgt_serializable2: Ghost.erased (tgt2 -> bool))
+    (#ps2: Ghost.erased (array_group_parser_spec t2 tgt_size2 tgt_serializable2))
+    (#impl_tgt2: Type0)
+    (#r2: rel impl_tgt2 tgt2)
+    (pa2: impl_zero_copy_array_group cbor_array_iterator_match ps2 r2)
+: impl_zero_copy_array_group #cbor_array_iterator_t cbor_array_iterator_match #(array_group_choice (Ghost.reveal t1) (Ghost.reveal t2)) #(tgt1 `either` tgt2) #(ag_spec_choice_size (Ghost.reveal tgt_size1) (Ghost.reveal tgt_size2)) #(ag_spec_choice_serializable (Ghost.reveal tgt_serializable1) (Ghost.reveal tgt_serializable2)) (array_group_parser_spec_choice (Ghost.reveal ps1) (Ghost.reveal ps2) (ag_spec_choice_size (Ghost.reveal tgt_size1) (Ghost.reveal tgt_size2)) (ag_spec_choice_serializable (Ghost.reveal tgt_serializable1) (Ghost.reveal tgt_serializable2))) #(impl_tgt1 `either` impl_tgt2) (rel_either r1 r2)
+=
+  (pc: _)
+  (#gc: _)
+  (#p: _)
+  (#l: _)
+{
+  let c0 = !pc;
+  let test1 = v1 pc;
+  Trade.elim _ _;
+  pc := c0;
+  if (test1) {
+    let w1 = pa1 pc;
+    with z1 . assert (r1 w1 z1);
+    let res : either impl_tgt1 impl_tgt2 = Inl w1;
+    Trade.rewrite_with_trade (r1 w1 z1) (rel_either r1 r2 res (Inl z1));
+    Trade.trans _ (r1 w1 z1) _;
+    res
+  } else {
+    let w2 = pa2 pc;
+    with z2 . assert (r2 w2 z2);
+    let res : either impl_tgt1 impl_tgt2 = Inr w2;
+    Trade.rewrite_with_trade (r2 w2 z2) (rel_either r1 r2 res (Inr z2));
+    Trade.trans _ (r2 w2 z2) _;
+    res
+  }
+}
+```
